Splinter/Journal/AllocationJournalRefinement.i.dfy
@@ -37,168 +37,111 @@ module AllocationJournalRefinment {
     && (forall addr | addr in addrs :: !allocator.CanAllocate(addr))
   }
 
-  // TODO(Jialin): bad name?
   predicate MiniAllocatorFollowfreshestRec(freshestRec: Pointer, allocator: MiniAllocator)
   {
-    // if freshestRec.None? then allocator.curr.None?
-    // else if freshestRec.Some? && allocator.curr.Some? 
-    // then allocator.MinAddr(freshestRec.value.NextPage())
-    // else true
-    && (freshestRec.None? ==> allocator.curr.None?)
-    && (freshestRec.Some? && allocator.curr.Some? ==> 
-      && var nextAddr := freshestRec.value.NextPage();
-      && allocator.MinAddr(nextAddr))
+    && (allocator.curr.Some? ==> 
+      && freshestRec.Some?
+      && freshestRec.value.au == allocator.curr.value)
   }
 
-  predicate InternalAUPagesFullyLinked(dv: DiskView, first: AU)
+  predicate {:opaque} InternalAUPagesFullyLinked(dv: DiskView, first: AU)
   {
     && (forall addr | addr in dv.entries && addr.au != first :: AUPagesLinkedTillFirstInOrder(dv, addr))
-    // forall addr | addr in addrs && addr.au != first :: AUPagesLinkedInOrder(dv, addr)
   }
 
   predicate Inv(v: Variables)
   {
+    && v.WF()
     && LR.Inv(v.journal)
-    // relationship between lsnAddrIndex and lsnAUIndex
     && AddrIndexConsistentWithAUIndex(v.journal.lsnAddrIndex, v.lsnAUIndex)
-    // relationship between lsnAddrIndex and miniAllocator status
     && JournalPagesNotFree(v.journal.lsnAddrIndex.Values, v.miniAllocator)
-    // relationship between journal freshestRec and miniAllocator
     && MiniAllocatorFollowfreshestRec(GetTj(v).freshestRec, v.miniAllocator)
     // constraints on page links within an AU
     // when one follows the prior link of a page within any AU except first
     // it will observe a link that's strictly decreasing and links down to page 0
     && InternalAUPagesFullyLinked(GetTj(v).diskView, v.first)
-
-    // To be deleted
-    // && (forall addr | addr in v.journal.lsnAddrIndex.Values :: 
-    //   && addr.au in v.lsnAUIndex.Values
-    //   && !v.miniAllocator.CanAllocate(addr))
-    // NOTE: may need to change to diskview for easier proof?
-    // && (forall addr | addr in v.journal.lsnAddrIndex.Values && addr.au != v.first ::
-    //   && AUPagesLinkedInOrder(v.journal.journal.truncatedJournal.diskView, addr))
   }
 
   lemma InternalJournalMarshalRefines(v: Variables, v': Variables, lbl: TransitionLabel, step: Step)
     requires Inv(v)
     requires InternalJournalMarshal(v, v', lbl, step)
     ensures L.InternalJournalMarshal(I(v), I(v'), lbl.I(), step.cut, step.addr)
-    ensures Inv(v')
+    ensures LR.Inv(v'.journal)
   {
     assert LR.Inv(v.journal);
+    if step.addr in v.journal.lsnAddrIndex.Values {
+      assert false;
+    }
     LR.InvNextMarshalStep(I(v), I(v'), lbl.I(), step.cut, step.addr);
-    assert LR.Inv(v'.journal);
+  }
 
-    assert v.miniAllocator.MinAddr(step.addr); // 
-    
-    assert LR.IndexDomainValid(v'.journal.lsnAddrIndex, GetTj(v')); // from LR.Inv
+  lemma AUPagesLinkedTillFirstInOrderInc(dv: DiskView, addr: Address, prior: Address)
+    requires addr == prior.NextPage()
+    requires dv.Decodable(Some(addr))
+    requires dv.entries[addr].CroppedPrior(dv.boundaryLSN) == Some(prior)
+    requires AUPagesLinkedTillFirstInOrder(dv, prior)
+    ensures AUPagesLinkedTillFirstInOrder(dv, addr)
+  {
+  }
+
+  lemma InternalJournalMarshalInv(v: Variables, v': Variables, lbl: TransitionLabel, step: Step)
+    requires Inv(v)
+    requires LR.Inv(v'.journal)
+    requires InternalJournalMarshal(v, v', lbl, step)
+    ensures Inv(v')
+  {
+    assert v.WF();
     var discardmsgs := v.journal.journal.unmarshalledTail.DiscardRecent(step.cut);
+    assert LR.IndexDomainValid(v'.journal.lsnAddrIndex, GetTj(v')); // from LR.Inv
     assert LikesJournal.LsnDisjoint(v.lsnAUIndex.Keys, discardmsgs) by {
       LR.reveal_IndexDomainValid();
     }
     assert v'.lsnAUIndex.Values == v.lsnAUIndex.Values + {step.addr.au};
     assert v'.journal.lsnAddrIndex.Values == v.journal.lsnAddrIndex.Values + {step.addr};
+    assert v'.WF();
+
     assert AddrIndexConsistentWithAUIndex(v'.journal.lsnAddrIndex, v'.lsnAUIndex);
-
-    // verifies just takes a while
-    assume JournalPagesNotFree(v'.journal.lsnAddrIndex.Values, v'.miniAllocator);
-
-    // assert MiniAllocatorFollowfreshestRec(GetTj(v).freshestRec, v.miniAllocator);
-    // assert GetTj(v).freshestRec.None? ==> v.miniAllocator.curr.None?;
-    // takes way too long to verify
-
-    assume MiniAllocatorFollowfreshestRec(GetTj(v').freshestRec, v'.miniAllocator);
-    // assert InternalAUPagesFullyLinked(GetTj(v').diskView, v'.first);
-
-    assert GetTj(v').diskView == GetTj(v).diskView.(entries :=
-      GetTj(v).diskView.entries[step.addr := 
-      LinkedJournal.JournalRecord(discardmsgs, GetTj(v).freshestRec)]);
-
-    forall addr | addr in GetTj(v').diskView.entries && addr.au != v'.first 
-      ensures AUPagesLinkedTillFirstInOrder(GetTj(v').diskView, addr)
+    forall addr | addr in v'.journal.lsnAddrIndex.Values
+      ensures !v'.miniAllocator.CanAllocate(addr)
     {
-      if addr in GetTj(v).diskView.entries {
-        assert AUPagesLinkedTillFirstInOrder(GetTj(v).diskView, addr);
+      if addr == step.addr {
+        assert !v'.miniAllocator.CanAllocate(addr);
       } else {
-        assert addr == step.addr;
-        if GetTj(v).freshestRec.None? {
-          // Jialin: all these assumes are asserts but idk why they take so long to verify
-          assume v.miniAllocator.curr.None?; 
-          assume v.miniAllocator.allocs[addr.au].MinFreeAddr(addr);
-          assume v.miniAllocator.allocs[addr.au]
-          v.miniAllocator.allocs[addr.au].MinFreeAddrZeroLemma(addr); 
-          assert addr.page == 0;
-          assume false;
-        } else {
-          assume false;
-        }
-
-//  && var newAddr := GenericDisk.Address(addr.au, page);
-//       && var priorAddr := GenericDisk.Address(addr.au, page-1);
-//       && dv.Decodable(Some(newAddr))
-//       && dv.entries[newAddr].CroppedPrior(dv.boundaryLSN) == Some(priorAddr))
-//   }
-
-        // we know cropped prior is fine 
-
-        // assume false;
+        assert !v.miniAllocator.CanAllocate(addr);
       }
     }
 
+    assert JournalPagesNotFree(v'.journal.lsnAddrIndex.Values, v'.miniAllocator);
+    assert MiniAllocatorFollowfreshestRec(GetTj(v).freshestRec, v.miniAllocator);
+    assert MiniAllocatorFollowfreshestRec(GetTj(v').freshestRec, v'.miniAllocator);
 
+    reveal_InternalAUPagesFullyLinked();
 
+    forall addr | addr in GetTj(v').diskView.entries && addr.au != v'.first
+      ensures AUPagesLinkedTillFirstInOrder(GetTj(v').diskView, addr)
+    {
+      if addr == step.addr {
+        assert GetTj(v').diskView.entries[step.addr].CroppedPrior(GetTj(v').diskView.boundaryLSN) == GetTj(v).freshestRec;
+        assert ValidNextJournalAddr(v, step.addr);
+        
+        if v.miniAllocator.curr.None? {
+          assert AUPagesLinkedTillFirstInOrder(GetTj(v').diskView, addr);
+        } else {
+          assert GetTj(v).freshestRec.Some?;
+          assert addr == GetTj(v).freshestRec.value.NextPage();
+          assert GetTj(v').diskView.Decodable(Some(addr));
 
-    // // relationship between journal freshestRec and miniAllocator
-    // && MiniAllocatorFollowfreshestRec(GetTj(v).freshestRec, v.miniAllocator)
-    // // constraints on page links within an AU
-    // // when one follows the prior link of a page within any AU except first
-    // // it will observe a link that's strictly decreasing and links down to page 0
-    // && InternalAUPagesFullyLinked(GetTj(v).diskView, v.first)
-
-  
-    // assume false;
-
-    // forall addr | addr in v'.journal.lsnAddrIndex.Values && addr.au != v'.first
-    //   ensures AUPagesLinkedInOrder(v'.journal.journal.truncatedJournal.diskView, addr)
-    // {
-    //   if addr in v.journal.lsnAddrIndex.Values {
-    //     assert AUPagesLinkedInOrder(v'.journal.journal.truncatedJournal.diskView, addr);
-    //   } else {
-
-    //     assert addr == v'.journal.journal.truncatedJournal.freshestRec.value;
-    //     assert v'.journal.journal.truncatedJournal.diskView.entries[addr].CroppedPrior(v'.journal.journal.truncatedJournal.diskView.boundaryLSN) == v.journal.journal.truncatedJournal.freshestRec;
-
-    //     var fr := v.journal.journal.truncatedJournal.freshestRec;
-    //     if fr.None? {
-    //       // we need to prove that page # is 0
-
-    //       // cur.Some? 
-    //       // connect freshest rec 
-    //     }
-
-    //     // if no record, mini allocator can't have a curr
-    //     // 
-
-    //     // invariants on the state of mini allocator?
-
-
-    //     // assert fr.Some?;
-    //     // assume addr == GenericDisk.Address(fr.value.au, fr.value.page+1);
-    //     // assume v.journal.journal.truncatedJournal.freshestRec == Some(GenericDisk.Address(addr.au, addr.page-1));
-
-    //     assume false;
-    //   }
-    // }
-
-    assume false;
+          assert AUPagesLinkedTillFirstInOrder(GetTj(v).diskView, GetTj(v).freshestRec.value);
+          AUPagesLinkedTillFirstInOrderInc(GetTj(v').diskView, addr, GetTj(v).freshestRec.value);
+        }
+      } else {
+        assert AUPagesLinkedTillFirstInOrder(GetTj(v).diskView, addr);
+      }
+    }
   }
 
   lemma InitRefines()
   {
 
   }
-
-
-
-
 }
